improve proofs

flat.v
@@ -1,49 +1,436 @@
-From iris.program_logic Require Export weakestpre.
+From iris.program_logic Require Export auth weakestpre.
 From iris.proofmode Require Import invariants ghost_ownership.
 From iris.heap_lang Require Export lang.
 From iris.heap_lang Require Import proofmode notation.
 From iris.heap_lang.lib Require Import spin_lock.
-From flatcomb Require Import sync_stack.
-Import uPred.
+From iris.algebra Require Import upred frac agree excl dec_agree upred_big_op gset gmap.
+From iris.tests Require Import misc atomic treiber_stack.
 
-Section flat_combiner.
-  Context `{!heapG Σ, !lockG Σ} (N: namespace).
-  Implicit Types l : loc.
+Definition doOp : val :=
+  λ: "f" "p",
+     match: !"p" with
+       InjL "x" => "p" <- InjR ("f" "x")
+     | InjR "_" => #()
+     end.
 
-  Definition install: val :=
-    λ: "lcl" "req" "push",
-       match: !"lcl" with
-         SOME "o" => "o" <- InjL "req";; "o"
-       | NONE => let: "o" := ref (InjL "req") in
-                 "lcl" <- "o";;
-                 "push" "o";;
-                 "o"
-       end.
+Definition doOp' (f:val) : val :=
+  λ: "p",
+     match: !"p" with
+       InjL "x" => "p" <- InjR (f "x")
+     | InjR "_" => #()
+     end.
 
-  Definition doOp: val :=
-    λ: "f" "o",
-       match: !"o" with
-         InjL "req" => "o" <- InjR ("f" "req")
-       | InjR "_" => #()
-       end.
+Definition try_srv : val :=
+  λ: "lk" "s" "f",
+    if: try_acquire "lk"
+      then let: "hd" := !"s" in
+           let: "f'" := doOp "f" in
+           iter "hd" "f'";;
+           release "lk"
+      else #().
 
-  Definition loop: val :=
-    rec: "loop" "o" "f" "lock" "iter" :=
-      match: !"o" with
-        InjL "_" =>
-          if: CAS "lock" #false #true
-            then "iter" (doOp "f") ;; "lock" <- #false;; "loop" "o" "f" "lock" "iter"
-            else "loop" "o" "f" "lock" "iter"
-      | InjR "res" => "res"
-      end.
+Definition loop: val :=
+  rec: "loop" "f" "p" "s" "lk" :=
+    match: !"p" with
+    InjL "_" =>
+        try_srv "lk" "s" "f";;
+        "loop" "f" "p" "s" "lk"
+    | InjR "r" => "r"
+    end.
 
-  Definition flat: val :=
-    λ: "f",
-       let: "lock" := ref (#false) in
-       let: "lcl" := ref #0 in
-       let: "s" := mk_stack #() in
-       λ: "x",
-          let: "o" := install "x" (push "s") in
-          loop "o" "f" "lock" (iter "s").
+Definition install : val :=
+  λ: "x" "s",
+     let: "p" := ref (InjL "x") in
+     push "s" "p";;
+     "p".
 
-End flat_combiner.
+Definition mk_flat : val :=
+  λ: <>,
+   let: "lk" := newlock #() in
+   let: "s" := new_stack #() in
+   λ: "f",
+      λ: "x",
+         let: "p" := install "x" "s" in
+         loop "f" "p" "s" "lk".
+
+Global Opaque doOp try_srv install loop mk_flat.
+
+Definition reqR := prodR fracR (dec_agreeR val). (* request x should be kept same *)
+Definition toks : Type := gname * gname * gname * gname. (* a bunch of tokens to do state transition *)
+Definition tokmR := evmapR loc toks. (* tie each slot to tokens *)
+Definition reqmR := evmapR loc val. (* tie each slot to request value *)
+Class flatG Σ := FlatG {
+  req_G :> inG Σ reqR;
+  tok_G :> inG Σ (authR tokmR);
+}.
+
+Definition flatΣ : gFunctors :=
+  #[ GFunctor (constRF reqR);
+     GFunctor (constRF (authR tokmR))
+   ].
+
+Instance subG_flatΣ {Σ} : subG flatΣ Σ → flatG Σ.
+Proof. intros [?%subG_inG [?%subG_inG _]%subG_inv]%subG_inv. split; apply _. Qed.
+
+Section proof.
+  Context `{!heapG Σ, !lockG Σ, !evidenceG loc val Σ, !flatG Σ} (N : namespace).
+  Context (R: iProp Σ) (* private resource *)
+          (P: val → iProp Σ) (* common pre-cond *)
+          (Q: val → val → iProp Σ) (* common post-cond *)
+          `{∀ x, TimelessP (P x), ∀ x y, TimelessP (Q x y)}.
+
+  Definition init_s (ts: toks) := let '(_, γ1, γ3, _) := ts in (own γ1 (Excl ()) ★ own γ3 (Excl ()))%I.
+  Definition installed_s (ts: toks) (x: val) :=
+    let '(γx, γ1, _, γ4) := ts in (own γx ((1/2)%Qp, DecAgree x) ★ P x ★ own γ1 (Excl ()) ★ own γ4 (Excl ()))%I.
+  Definition received_s (ts: toks) (x: val) γr :=
+    let '(γx, _, _, γ4) := ts in (own γx ((1/2/2)%Qp, DecAgree x) ★ own γr (Excl ()) ★ own γ4 (Excl ()))%I.
+  Definition finished_s (ts: toks) (x y: val) :=
+    let '(γx, γ1, _, γ4) := ts in
+    (own γx ((1/2)%Qp, DecAgree x) ★ Q x y ★ own γ1 (Excl ()) ★ own γ4 (Excl ()))%I.
+
+  Definition evm := ev loc toks.
+  
+  (* p slot invariant *)
+  Definition p_inv (γm γr: gname) (v: val) :=
+    (∃ (ts: toks) (p : loc),
+       v = #p ★ evm γm p ts ★
+       ((* INIT *)
+        (∃ y: val, p ↦{1/2} InjRV y ★ init_s ts)∨
+        (* INSTALLED *)
+        (∃ x: val, p ↦{1/2} InjLV x ★ installed_s ts x) ∨
+        (* RECEIVED *)
+        (∃ x: val, p ↦{1/2} InjLV x ★ received_s ts x γr) ∨
+        (* FINISHED *)
+        (∃ x y: val, p ↦{1/2} InjRV y ★ finished_s ts x y)))%I.
+
+  Global Instance p_inv_timeless γm γr v: TimelessP (p_inv γm γr v).
+  Proof. rewrite /p_inv.  apply uPred.exist_timeless. destruct x as [[[? ?] ?] ?]. apply _. Qed.
+
+  Definition srv_stack_inv (γs γm γr: gname) (s: loc) := (∃ xs, is_stack' (p_inv γm γr) γs xs s)%I.
+
+  Definition srv_tokm_inv γm := (∃ m : tokmR, own γm (● m) ★ [★ map] p ↦ _ ∈ m, ∃ v, p ↦{1/2} v)%I.
+
+  Lemma install_push_spec
+        (Φ: val → iProp Σ)
+        (p: loc) (γs γm γr: gname) (ts: toks)
+        (s: loc) (x: val) :
+    heapN ⊥ N →
+    heap_ctx ★ inv N (srv_stack_inv γs γm γr s ★ srv_tokm_inv γm) ★
+    evm γm p ts ★ installed_s ts x ★
+    p ↦{1/2} InjLV x ★ ((∃ hd, evs γs hd #p) -★ Φ #())
+    ⊢ WP push #s #p {{ Φ }}.
+  Proof.
+    iIntros (HN) "(#Hh & #? & Hpm & Hs & Hp & HΦ)".
+    rewrite /srv_stack_inv.
+    iDestruct (push_spec N (p_inv γm γr) (fun v => (∃ hd, evs γs hd #p) ★ v = #())%I
+               with "[-HΦ]") as "Hpush"=>//.
+    - iFrame "Hh". iSplitL "Hp Hs Hpm"; last eauto.
+      iExists ts. iExists p. iSplit=>//. iFrame "Hpm".
+      iRight. iLeft. iExists x. iFrame.
+    - iApply wp_wand_r.
+      iSplitL "Hpush"; first done.
+      iIntros (?) "[? %]". subst.
+      by iApply "HΦ".
+  Qed.
+
+  Definition installed_recp (ts: toks) (x: val) :=
+    let '(γx, _, γ3, _) := ts in (own γ3 (Excl ()) ★ own γx ((1/2)%Qp, DecAgree x))%I.
+
+  Lemma install_spec
+        (Φ: val → iProp Σ)
+        (x: val) (γs γm γr: gname) (s: loc):
+    heapN ⊥ N →
+    heap_ctx ★ inv N (srv_stack_inv γs γm γr s ★ srv_tokm_inv γm) ★ P x ★
+    (∀ (p: loc) (ts: toks), installed_recp ts x -★ evm γm p ts -★(∃ hd, evs γs hd #p) -★ Φ #p)
+    ⊢ WP install x #s {{ Φ }}.
+  Proof.
+    iIntros (HN) "(#Hh & #? & Hpx & HΦ)".
+    wp_seq. wp_let. wp_alloc p as "Hl".
+    iApply pvs_wp.
+    iVs (own_alloc (Excl ())) as (γ1) "Ho1"; first done.
+    iVs (own_alloc (Excl ())) as (γ3) "Ho3"; first done.
+    iVs (own_alloc (Excl ())) as (γ4) "Ho4"; first done.
+    iVs (own_alloc (1%Qp, DecAgree x)) as (γx) "Hx"; first done.
+    iInv N as ">[Hrs Hm]" "Hclose".
+    iDestruct "Hm" as (m) "[Hm HRm]".
+    destruct (m !! p) eqn:Heqn.
+    - (* old name *)
+      iDestruct (big_sepM_delete (fun p _ => ∃ v : val, p ↦{1 / 2} v)%I m with "HRm") as "[Hp HRm]"=>//.
+      iDestruct "Hp" as (?) "Hp". iExFalso. iApply bogus_heap; last by iFrame "Hh Hl Hp". auto.
+    - (* fresh name *)
+      iDestruct (evmap_alloc _ _ _ m p (γx, γ1, γ3, γ4) with "[Hm]") as "==>[Hm1 Hm2]"=>//.
+      iDestruct "Hl" as "[Hl1 Hl2]".
+      iVs ("Hclose" with "[HRm Hm1 Hl1 Hrs]").
+      + iNext. iFrame. iExists ({[p := (1%Qp, DecAgree (γx, γ1, γ3, γ4))]} ⋅ m). iFrame.
+        rewrite <-(insert_singleton_op m)=>//.
+        iDestruct (big_sepM_insert _ m with "[-]") as "H"=>//.
+        iSplitL "Hl1"; last by iAssumption. eauto.
+      + iDestruct (pack_ev with "Hm2") as "Hev".
+        iDestruct (dup_ev with "Hev") as "==>[Hev1 Hev2]".
+        iDestruct (own_update with "Hx") as "==>[Hx1 Hx2]"; first by apply pair_l_frac_op_1'.
+        iVsIntro. wp_let. wp_bind ((push _) _).
+        iApply install_push_spec=>//.
+        iFrame "#". rewrite /evm /installed_s.
+        iFrame "Hev1 Hx1 Hpx Ho1 Ho4 Hl2".
+        iIntros "Hhd". wp_seq. iVsIntro.
+        iSpecialize ("HΦ" $! p (γx, γ1, γ3, γ4) with "[-Hev2 Hhd]")=>//.
+        { rewrite /installed_recp. iFrame. }
+        by iApply ("HΦ" with "Hev2").
+  Qed.
+
+  Lemma loop_iter_list_spec Φ (f: val) (s hd: loc) (γs γm γr: gname) xs:
+    heapN ⊥ N → (∀ x:val, {{ R ★ P x }} f x {{ v, R ★ Q x v }}) ★
+    heap_ctx ★ inv N (srv_stack_inv γs γm γr s ★ srv_tokm_inv γm) ★ own γr (Excl ()) ★ R ★
+    is_list' γs hd xs ★ (own γr (Excl ()) -★ R -★ Φ #())
+    ⊢ WP doOp f {{ f', WP iter #hd f' {{ Φ }} }}.
+  Proof.
+    iIntros (HN) "(#Hf & #? & #? & Ho2 & HR & Hlist' & HΦ)".
+    iApply pvs_wp.
+    iDestruct (dup_is_list' with "[Hlist']") as "==>[Hl1 Hl2]"; first by iFrame.
+    iDestruct (dup_is_list' with "[Hl2]") as "==>[Hl2 Hl3]"; first by iFrame.
+    iVsIntro. wp_seq.
+    iDestruct (iter_spec _ (p_inv γm γr) (fun v => v = #() ★ own γr (Excl ()) ★ R)%I γs s
+                         ((∀ x:val, {{ R ★ P x }} f x {{ v, R ★ Q x v }}) ★
+                          is_list' γs hd xs ★ own γr (Excl ()) ★ R)%I (srv_tokm_inv γm) xs hd
+                         (doOp' f) (doOp' f)
+                         with "[-Hl1 HΦ]") as "Hiter"=>//.
+    - rewrite /f_spec.
+      iIntros (Φ' p _ Hin) "(#Hh & #? & (#Hf & Hls & Ho2 & HR) & HΦ')".
+      wp_let. wp_bind (! _)%E. iInv N as ">[Hs Hm]" "Hclose".
+      iDestruct "Hs" as (xs' hd') "[Hhd [Hxs HRs]]".
+      iDestruct (dup_is_list' with "[Hls]") as "==>[Hls1 Hls2]"; first by iFrame.
+      iDestruct "HRs" as (m) "[Hom HRs]".
+      iDestruct (access with "[Hom HRs Hls1]") as (hd'' [q x]) "[Hrest [Hhd'' [% Hom]]]"=>//; first by iFrame.
+      iDestruct "Hhd''" as "(% & H & Hphd)". inversion H2. subst.
+      iDestruct "H" as (ts p'') "[% [Hev [Hp | [Hp | [Hp | Hp]]]]]"; subst.
+      + iDestruct "Hp" as (y) "(Hp & Hs)".
+        wp_load. iVs ("Hclose" with "[-HΦ' Ho2 HR Hls2]").
+        { iNext. iFrame. iExists xs', hd'.
+          iFrame "Hhd Hxs". iExists m.
+          iFrame "Hom". iDestruct (big_sepM_delete _ m with "[Hrest Hphd Hev Hp Hs]") as "?"=>//.
+          iFrame. iExists #p''. iSplitR; first done. iExists ts, p''.
+          iSplitR; first done. iFrame. iLeft. iExists y. iFrame. }
+        iVsIntro. wp_match. iApply "HΦ'". by iFrame.
+      + iDestruct "Hp" as (x') "(Hp & Hs)".
+        wp_load. destruct ts as [[[γx γ1] γ3] γ4].
+        iDestruct "Hs" as "(Hx & Hpx & Ho1 & Ho4)".
+        iDestruct (dup_ev with "Hev") as "==>[Hev1 Hev2]".
+        iAssert (|=r=> own γx (((1/2/2)%Qp, DecAgree x') ⋅
+                               ((1/2/2)%Qp, DecAgree x')))%I with "[Hx]" as "==>[Hx1 Hx2]".
+        { iDestruct (own_update with "Hx") as "?"; last by iAssumption.
+          rewrite -{1}(Qp_div_2 (1/2)%Qp).
+          by apply pair_l_frac_op'. }
+        iVs ("Hclose" with "[-Hls2 Ho1 Hx2 HR Hev2 Hpx HΦ']").
+        { iNext. iFrame. iExists xs', hd'.
+          iFrame "Hhd Hxs". iExists m.
+          iFrame "Hom". iDestruct (big_sepM_delete _ m with "[-]") as "?"=>//.
+          simpl. iFrame. iExists #p''. iSplitR; auto. rewrite /allocated.
+          iExists (γx, γ1, γ3, γ4), p''. iSplitR; auto.
+          iFrame. iRight. iRight. iLeft. iExists x'. iFrame. }
+        iVsIntro. wp_match.
+        wp_bind (f _). iApply wp_wand_r. iSplitL "Hpx HR".
+        { iApply "Hf". iFrame. }
+        iIntros (v) "[HR HQ]".
+        wp_value. iVsIntro. iInv N as ">[Hs Hm]" "Hclose".
+        iDestruct "Hs" as (xs'' hd''') "[Hhd [Hxs HRs]]".
+        iDestruct "HRs" as (m') "[Hom HRs]".
+        iDestruct (dup_is_list' with "[Hls2]") as "==>[Hls2 Hls3]"; first by iFrame.
+        iDestruct (access with "[Hom HRs Hls2]") as (hd'''' [? ?]) "[Hrest [Hhd'' [% Hom]]]"=>//;
+         first by iFrame.
+        iDestruct "Hhd''" as "(% & H & Hphd)". inversion H4. subst.
+        iDestruct "H" as ([[[γx' γ1'] γ3'] γ4'] p'''') "[% [Hev Hps]]".
+        inversion H5. subst.
+        destruct (decide (γ1 = γ1' ∧ γx = γx' ∧ γ3 = γ3' ∧ γ4 = γ4')) as [[? [? [? ?]]]|Hneq]; subst.
+        {
+          iDestruct "Hps" as "[Hp | [Hp | [Hp | Hp]]]".
+          * iDestruct "Hp" as (?) "(_ & Ho1' & _)".
+            iApply excl_falso. iFrame.
+          * iDestruct "Hp" as (?) "(_ & _ & _ & Ho1' & _)".
+            iApply excl_falso. iFrame.
+          * iDestruct "Hp" as (x5) "(Hp & Hx & Ho2 & Ho4)".
+            iDestruct "Hm" as (m2) "[Hom2 HRm]".
+            destruct (m2 !! p'''') eqn:Heqn.
+            {
+              iDestruct (big_sepM_delete _ m2 with "HRm") as "[HRk HRm]"=>//.
+              iDestruct "HRk" as (?) "HRk".
+              iDestruct (heap_mapsto_op_1 with "[HRk Hp]") as "[% Hp]"; first by iFrame.
+              rewrite Qp_div_2. wp_store.
+              (* now close the invariant *)
+              iDestruct (m_frag_agree with "[Hx Hx2]") as "==>[Hx %]"; first iFrame.
+              subst. rewrite Qp_div_2. iVs ("Hclose" with "[-HΦ' Ho2 HR Hls3]").
+              { iNext. iDestruct "Hp" as "[Hp1 Hp2]".
+                iAssert (srv_tokm_inv γm) with "[Hp1 HRm Hom2]" as "HRm".
+                { iExists m2. iFrame. iApply (big_sepM_delete _ m2)=>//.
+                  iFrame. eauto. }
+                iFrame. iExists xs''. iFrame. iExists hd'''. iFrame.
+                iExists m'. iFrame.
+                iDestruct (big_sepM_delete _ m' with "[-]") as "?"=>//.
+                { simpl. iFrame. iExists #p''''.
+                  iSplitR; first auto. iExists (γx', γ1', γ3', γ4'), p''''.
+                  iSplitR; first auto. iFrame "Hev". iRight. iRight.
+                  iRight. iExists x5, v. iFrame.
+                }
+              }
+              iApply "HΦ'". by iFrame.
+            }
+            { iExFalso. iApply (map_agree_none' _ _ _ m2)=>//. iFrame. }
+          * iDestruct "Hp" as (? ?) "(_ & _ & _ & Ho1' & _)".
+            iApply excl_falso. iFrame.
+        }
+        { iDestruct (ev_agree with "[Hev2 Hev]") as "==>[_ [_ %]]"; first iFrame.
+          inversion H6. subst. by contradiction Hneq. }
+      + destruct ts as [[[γx γ1] γ3] γ4]. iDestruct "Hp" as (y) "(_ & _ & Ho2' & _)".
+        iApply excl_falso. iFrame.
+      + destruct ts as [[[γx γ1] γ3] γ4]. iDestruct "Hp" as (x' y) "(Hp & Hx & HQxy & Ho1 & Ho4)".
+        wp_load. iVs ("Hclose" with "[-HΦ' HR Ho2 Hls2]").
+        { iNext. iFrame. iExists xs', hd'.
+          iFrame "Hhd Hxs". iExists m.
+          iFrame "Hom". iDestruct (big_sepM_delete _ m with "[-]") as "?"=>//.
+          iFrame. iExists #p''. iSplitR; first auto. iExists (γx, γ1, γ3, γ4), p''.
+          iSplitR; auto. iFrame. iRight. iRight. iRight. iExists x', y. iFrame. }
+        iVsIntro. wp_match. iApply "HΦ'". by iFrame.
+    - apply to_of_val.
+    - rewrite /srv_stack_inv. iFrame "#". iFrame. iIntros "[_ (? & ? & ?)]". by iFrame.
+    - iApply wp_wand_r. iSplitL "Hiter"; first done.
+      iIntros (?) "[% [Ho2 HR]]". subst. iApply ("HΦ" with "Ho2 HR").
+  Qed.
+
+  Definition own_γ3 (ts: toks) := let '(_, _, γ3, _) := ts in own γ3 (Excl ()).
+  Definition finished_recp (ts: toks) (x y: val) :=
+    let '(γx, _, _, _) := ts in (own γx ((1 / 2)%Qp, DecAgree x) ★ Q x y)%I.
+
+  Lemma try_srv_spec Φ (s: loc) (lk: val) (f: val)
+        (γs γr γm γlk: gname):
+    heapN ⊥ N → (∀ x:val, {{ R ★ P x }} f x {{ v, R ★ Q x v }}) ★
+    heap_ctx ★ inv N (srv_stack_inv γs γm γr s ★ srv_tokm_inv γm) ★
+    is_lock N γlk lk (own γr (Excl ()) ★ R) ★ Φ #()
+    ⊢ WP try_srv lk #s f {{ Φ }}.
+  Proof.
+    iIntros (?) "(#? & #? & #? & #? & HΦ)".
+    wp_seq. wp_let. wp_let.
+    wp_bind (try_acquire _). iApply try_acquire_spec.
+    iFrame "#". iSplit; last by wp_if.
+    (* acquired the lock *)
+    iIntros "Hlocked [Ho2 HR]".
+    wp_if. wp_bind (! _)%E.
+    iInv N as ">[H Hm]" "Hclose".
+    iDestruct "H" as (xs' hd') "[Hs [Hxs HRs]]".
+    wp_load. iDestruct (dup_is_list' with "[Hxs]") as "==>[Hxs1 Hxs2]"; first by iFrame.
+    iVs ("Hclose" with "[Hs Hxs1 HRs Hm]").
+    { iNext. iFrame. iExists xs', hd'. by iFrame. }
+    iVsIntro. wp_let. wp_bind (doOp f).
+    iApply wp_wand_r. iSplitL "HR Ho2 Hxs2".
+    { iApply (loop_iter_list_spec (fun v => own γr (Excl ()) ★ R ★ v = #()))%I=>//.
+      iFrame "#". iFrame. iIntros "? ?". by iFrame. }
+    iIntros (f') "Hf'".
+    wp_let. wp_bind ((iter _) _).
+    iApply wp_wand_r. iSplitL "Hf'"; first iApply "Hf'".
+    iIntros (?) "[Ho2 [HR %]]". subst.
+    wp_seq. iApply release_spec.
+    iFrame "#". iFrame.
+  Qed.
+    
+  Lemma loop_spec Φ (p s: loc) (lk: val) (f: val)
+        (γs γr γm γlk: gname) (ts: toks):
+    heapN ⊥ N → (∀ x:val, {{ R ★ P x }} f x {{ v, R ★ Q x v }}) ★
+    heap_ctx ★ inv N (srv_stack_inv γs γm γr s ★ srv_tokm_inv γm) ★
+    is_lock N γlk lk (own γr (Excl ()) ★ R) ★
+    own_γ3 ts ★ evm γm p ts ★
+    (∃ hd, evs γs hd #p) ★ (∀ x y, finished_recp ts x y -★ Φ y)
+    ⊢ WP loop f #p #s lk {{ Φ }}.
+  Proof.
+    iIntros (HN) "(#Hf & #Hh & #? & #? & Ho3 & Hev & Hhd & HΦ)".
+    iLöb as "IH". wp_rec. repeat wp_let.
+    wp_bind (! _)%E. iInv N as ">[Hinv ?]" "Hclose".
+    iDestruct "Hinv" as (xs hd) "[Hs [Hxs HRs]]".
+    iDestruct "HRs" as (m) "[Hom HRs]".
+    iDestruct "Hhd" as (hdp ?) "Hhd".
+    destruct (m !! hdp) eqn:Heqn.
+    - iDestruct (big_sepM_delete _ m with "HRs") as "[Hp Hrs]"=>//.
+      iDestruct "Hp" as (?) "[% [Hpr ?]]"; subst.
+      iDestruct "Hpr" as (ts' p') "(% & Hp' & Hp)".
+      subst. iDestruct (map_agree_eq' _ _ γs m with "[Hom Hhd]") as "(Hom & Hhd & %)"=>//.
+      { iFrame. rewrite /ev. eauto. }
+      inversion H2. subst.
+      iDestruct (ev_agree with "[Hev Hp']") as "==>[Hγs2 [Hγs %]]"; first iFrame. subst.
+      destruct ts as [[[γx γ1] γ3] γ4].
+      iDestruct "Hp" as "[Hp | [Hp | [ Hp | Hp]]]".
+      + iDestruct "Hp" as (?) "(_ & _ & Ho3')".
+        iApply excl_falso. iFrame.
+      + iDestruct "Hp" as (x) "(Hp & Hx & Ho1 & Ho4)".
+        wp_load. iVs ("Hclose" with "[-Hγs2 Ho3 HΦ Hhd]").
+        { iNext. iFrame. iExists xs, hd. iFrame. iExists m. iFrame.
+          iDestruct (big_sepM_delete _ m with "[-]") as "?"=>//.
+          iFrame. iExists #p'. iSplitR; first auto. iExists (γx, γ1, γ3, γ4), p'.
+          iSplitR; first auto. iFrame.
+          iRight. iLeft. iExists x.
+          iFrame. }
+        iVsIntro. wp_match.
+        wp_bind (try_srv _ _ _). iApply try_srv_spec=>//.
+        iFrame "#". wp_seq.
+        iAssert (∃ hd, evs γs hd #p')%I with "[Hhd]" as "Hhd"; eauto.
+        by iApply ("IH" with "Ho3 Hγs2 Hhd").
+      + iDestruct "Hp" as (x) "(Hp & Hx & Ho2 & Ho4)".
+        wp_load.
+        iVs ("Hclose" with "[-Hγs Ho3 HΦ Hhd]").
+        { iNext. iFrame. iExists xs, hd. iFrame. iExists m. iFrame.
+          iDestruct (big_sepM_delete _ m with "[-]") as "?"=>//.
+          iFrame. iExists #p'. iSplitR; auto. iExists (γx, γ1, γ3, γ4), p'.
+          iSplitR; first auto. iFrame.
+          iRight. iRight. iLeft. iExists x. iFrame.
+        }
+        iVsIntro. wp_match.
+        wp_bind (try_srv _ _ _). iApply try_srv_spec=>//.
+        iFrame "#". wp_seq.
+        iAssert (∃ hd, evs γs hd #p')%I with "[Hhd]" as "Hhd"; eauto.
+        by iApply ("IH" with "Ho3 Hγs Hhd").
+      + iDestruct "Hp" as (x y) "(Hp & Hx & HQ & Ho1 & Ho4)".
+          wp_load.
+          iVs ("Hclose" with "[-Hγs Ho4 HΦ Hx HQ]").
+          { iNext. iFrame. iExists xs, hd. iFrame. iExists m. iFrame.
+            iDestruct (big_sepM_delete _ m with "[-]") as "?"=>//.
+            iFrame. iExists #p'. iSplitR; auto. iExists (γx, γ1, γ3, γ4), p'.
+            iSplitR; first auto. iFrame.
+            iLeft. iExists y. iFrame. }
+          iVsIntro. wp_match. iApply ("HΦ" with "[-]"). iFrame.
+    - iExFalso. iApply (map_agree_none' _ _ _ m)=>//. iFrame "Hom".
+      rewrite /ev. eauto.
+  Qed.
+
+  Definition is_flatter (fl: val) :=
+    (∀ f:val , WP fl f {{ f', □ ((∀ x:val, {{ R ★ P x }} f x {{ v, R ★ Q x v }}) →
+                                 (∀ x:val, {{ P x }} f' x {{ v, Q x v }}))}})%I.
+
+  Lemma mk_flat_spec:
+    ∀ (Φ: val → iProp Σ),
+      heapN ⊥ N →
+      heap_ctx ★ R ★ (∀ fl, is_flatter fl -★ Φ fl) ⊢ WP mk_flat #() {{ Φ }}.
+  Proof.
+    iIntros (Φ HN) "(#Hh & HR & HΦ)".
+    iVs (own_alloc (Excl ())) as (γr) "Ho2"; first done.
+    iVs (own_alloc (● (∅: tokmR) ⋅ ◯ ∅)) as (γm) "[Hm _]"; first by rewrite -auth_both_op.
+    iAssert (srv_tokm_inv γm) with "[Hm]" as "Hm"; first eauto.
+    { iExists ∅. iFrame. by rewrite big_sepM_empty. }
+    wp_seq. wp_bind (newlock _).
+    iApply (newlock_spec _ (own γr (Excl ()) ★ R))%I=>//.
+    iFrame "Hh Ho2 HR". iIntros (lk γlk) "#Hlk".
+    wp_let. wp_bind (new_stack _).
+    iApply (new_stack_spec' _ (p_inv γm γr))=>//.
+    iFrame "Hh Hm". iIntros (γ s) "#Hss".
+    wp_let. iVsIntro. iApply "HΦ". rewrite /is_flatter. iIntros (f). wp_let.
+    iVsIntro. iAlways. iIntros "#Hf".
+    iIntros (x) "!# Hp". wp_let.
+    wp_bind ((install _) _).
+    iApply install_spec=>//.
+    iFrame "#". iFrame "Hp". iIntros (p [[[γx γ1] γ3] γ4]) "[Ho3 Hx] Hev Hhd".
+    wp_let. iApply loop_spec=>//.
+    iFrame "#". iFrame.
+    iIntros (? ?) "[Hx' HQ]".
+    destruct (decide (x = a)) as [->|Hneq]; first done.
+    { iExFalso. iCombine "Hx" "Hx'" as "Hx".
+      iDestruct (own_valid with "Hx") as %[_ H1].
+      rewrite pair_op //= dec_agree_ne in H1=>//.
+    }
+  Qed.
+
+End proof.
